Use names from the book to decrease mental overhead

Chapter3.thy
@@ -1,5 +1,5 @@
 theory Chapter3
-imports Main
+imports Main HOL.Fun
 begin
 
 (* Section 3.1 *)
@@ -11,25 +11,25 @@ fun abc_var :: "var_name" where
 "abc_var = VarName ''abc''"
 *)
 
-datatype arith_expr =
+datatype aexp =
     N int
   | V var_name
-  | Plus arith_expr arith_expr
+  | Plus aexp aexp
 
 type_synonym val   = int
 type_synonym state = "var_name \<Rightarrow> val"
 
-fun arith_expr_value :: "arith_expr \<Rightarrow> state \<Rightarrow> val" where
-"arith_expr_value (N n)      _ = n"   |
-"arith_expr_value (V v)      s = s v" |
-"arith_expr_value (Plus x y) s = arith_expr_value x s + arith_expr_value y s"
+fun aval :: "aexp \<Rightarrow> state \<Rightarrow> val" where
+"aval (N n)      _ = n"   |
+"aval (V v)      s = s v" |
+"aval (Plus x y) s = aval x s + aval y s"
 
-value "arith_expr_value (Plus (N 3) (V (VarName ''x''))) ((\<lambda> _. 0) (VarName ''x'' := 5))"
+value "aval (Plus (N 3) (V (VarName ''x''))) ((\<lambda> _. 0) (VarName ''x'' := 5))"
 
 fun undef_state :: "state" where
 "undef_state (VarName []) = 1"
 
-value "arith_expr_value (Plus (N 3) (V (VarName ''x''))) undef_state"
+value "aval (Plus (N 3) (V (VarName ''x''))) undef_state"
 
 (*fun mk_state :: "int \<Rightarrow> (string * int) list \<Rightarrow> state" where
 "mk_state initial bindings = "
@@ -38,7 +38,7 @@ value "arith_expr_value (Plus (N 3) (V (VarName ''x''))) undef_state"
 fun init_state :: "state" where
 "init_state _ = 0"
 
-fun asimp_const :: "arith_expr \<Rightarrow> arith_expr" where
+fun asimp_const :: "aexp \<Rightarrow> aexp" where
 "asimp_const (N n) = N n" |
 "asimp_const (V v) = V v" |
 "asimp_const (Plus x y) =
@@ -46,43 +46,43 @@ fun asimp_const :: "arith_expr \<Rightarrow> arith_expr" where
    (N x', N y') \<Rightarrow> N (x' + y') |
    (x',   y')   \<Rightarrow> Plus x' y')"
 
-lemma asimp_const_preserves_semantics : "arith_expr_value (asimp_const e) s = arith_expr_value e s"
+lemma asimp_const_preserves_semantics : "aval (asimp_const e) s = aval e s"
 apply(induction e)
-apply(auto split: arith_expr.split)
+apply(auto split: aexp.split)
 done
 
-fun plus :: "arith_expr \<Rightarrow> arith_expr \<Rightarrow> arith_expr" where
+fun plus :: "aexp \<Rightarrow> aexp \<Rightarrow> aexp" where
 "plus (N x) (N y) = N (x + y)"                               |
 "plus (N x) y     = (if x = 0 then y else Plus (N x) y)"     |
 "plus x     (N y) = (if y = 0 then x else Plus x     (N y))" |
 "plus x     y     = Plus x y"
 
-lemma plus_adds : "arith_expr_value (plus e1 e2) s = arith_expr_value e1 s + arith_expr_value e2 s"
+lemma plus_adds : "aval (plus e1 e2) s = aval e1 s + aval e2 s"
 apply(induction e1 e2 rule: plus.induct)
 apply(auto)
 done
 
-fun asimp :: "arith_expr \<Rightarrow> arith_expr" where
+fun asimp :: "aexp \<Rightarrow> aexp" where
 "asimp (N x)      = N x" |
 "asimp (V x)      = V x" |
 "asimp (Plus x y) = plus x y"
 
-lemma "arith_expr_value (asimp e) s = arith_expr_value e s"
+lemma "aval (asimp e) s = aval e s"
 apply(induction e)
 apply(auto simp add: plus_adds)
 done
 
 (* Exercise 3.1 *)
 
-fun optimal :: "arith_expr \<Rightarrow> bool" where
+fun optimal :: "aexp \<Rightarrow> bool" where
 "optimal (N _)              = True"  |
 "optimal (V _)              = True"  |
 "optimal (Plus (N _) (N _)) = False" |
 "optimal (Plus x     y)     = (optimal x \<and> optimal y)"
 
-theorem asimp_const_is_optimal : "optimal (asimp_const e)"
+theorem "optimal (asimp_const e)"
 apply(induction e)
-apply(auto split: arith_expr.split)
+apply(auto split: aexp.split)
 done
 
 (* Exercise 3.2 *)
@@ -92,23 +92,33 @@ value "None"
 value "fst"
 value "let (x, y) = (1, 2 :: int) in x + y"
 
-datatype arith_expr_simplified =
+datatype aexp_simplified =
     Constant int
-  | VanillaTerm arith_expr
+  | VanillaTerm aexp
   (* Term plus some constant *)
-  | Term arith_expr int (* integer is always nonzero *) 
+  | Term aexp int (* integer is always nonzero *) 
 
-fun unsimplify :: "arith_expr_simplified \<Rightarrow> arith_expr" where
+fun unsimplify :: "aexp_simplified \<Rightarrow> aexp" where
 "unsimplify (Constant n)    = N n" |
 "unsimplify (VanillaTerm e) = e"   |
 "unsimplify (Term e n)      = Plus e (N n)"
 
-fun addConstant :: "int \<Rightarrow> arith_expr_simplified \<Rightarrow> arith_expr_simplified" where
-"addConstant n (Constant m)    = Constant (n + m)"                            |
+fun addConstant :: "int \<Rightarrow> aexp_simplified \<Rightarrow> aexp_simplified" where
+"addConstant n e =
+ (if n = 0
+  then e
+  else case e of
+    Constant m    \<Rightarrow> Constant (n + m) |
+    VanillaTerm e \<Rightarrow> Term e n         |
+    Term e m      \<Rightarrow> Term e (n + m)
+  )"
+(*
+  "addConstant n (Constant m)    = Constant (n + m)"                            |
 "addConstant n (VanillaTerm e) = (if n = 0 then VanillaTerm e else Term e n)" |
 "addConstant n (Term e m)      = Term e (n + m)"
+*)
 
-fun full_asimp_helper :: "arith_expr \<Rightarrow> arith_expr_simplified" where
+fun full_asimp_helper :: "aexp \<Rightarrow> aexp_simplified" where
 "full_asimp_helper (N n)      = Constant n"        |
 "full_asimp_helper (V v)      = VanillaTerm (V v)" |
 "full_asimp_helper (Plus x y) =
@@ -119,19 +129,19 @@ fun full_asimp_helper :: "arith_expr \<Rightarrow> arith_expr_simplified" where
    (VanillaTerm e, Term e' m)      \<Rightarrow> Term (Plus e e') m      |
    (Term e n,      VanillaTerm e') \<Rightarrow> Term (Plus e e') n      |
    (Term e n,      Term e' m)      \<Rightarrow> Term (Plus e e') (n + m))"
-
-fun full_asimp :: "arith_expr \<Rightarrow> arith_expr" where
-"full_asimp e = unsimplify (full_asimp_helper e)"
+   
+fun full_asimp :: "aexp \<Rightarrow> aexp" where
+"full_asimp x = (unsimplify \<circ> full_asimp_helper) x" (* Enter composition via \circ *)
 
 lemma addConstant_preserves_semantics : 
-  "arith_expr_value (unsimplify (addConstant n e)) s = n + arith_expr_value (unsimplify e) s"
+  "aval (unsimplify (addConstant n e)) s = n + aval (unsimplify e) s"
 apply(induction e)
-apply(auto split: arith_expr_simplified.split)
+apply(auto split: aexp_simplified.split)
 done
 
-theorem full_asimp_preserves_semantics : "arith_expr_value (full_asimp e) s = arith_expr_value e s"
+theorem full_asimp_preserves_semantics : "aval (full_asimp e) s = aval e s"
 apply(induction e)
-apply(auto split: arith_expr_simplified.split simp add: addConstant_preserves_semantics)
+apply(auto split: aexp_simplified.split simp add: addConstant_preserves_semantics)
 (* apply(auto simp add: split_def Let_def split: option.split) (* split_def is needed to expand cases over tuples *) *)
 done
 
